act1/theories/Syntax.v
@@ -30,68 +30,51 @@ Canonical CH_var_eqType := EqType _ CH.var_eqMixin.
 
 (* expressions and processes *)
 
+(* expressions *)
+
 Inductive exp : Set :=
   | tt
   | ff
+  | one
   | V of evar
 .
 
-(* CoInductive just because we don't need an induction principle *)
-(* CoInductive polarity := Pos | Neg. (* TODO really replace this by bool *) *)
-(* Definition dual_pol p := if p is Pos then Neg else Pos. *)
+Coercion V : evar >-> exp.
 
-(* Definition eq_polarity (p p' : polarity) : bool := *)
-(*   match p, p' with *)
-(*   | Pos, Pos *)
-(*   | Neg, Neg => true *)
-(*   | _, _ => false *)
-(*   end. *)
+(* A simple extension would be to add simple computation to
+expressions. This would require adding reductions to expressions. And
+proving these reductions are type preserving etc.
 
-(* Lemma polarity_reflect : Equality.axiom eq_polarity. *)
-(* Proof. *)
-(*     by do !case ; constructor. *)
-(* Qed. *)
+For example, implementing 'not' that takes a boolean and returns its
+negation would be a simple computation rule.
+*)
 
-(* Definition polarity_eqMixin := EqMixin polarity_reflect. *)
-(* Canonical polarity_eqType := EqType _ polarity_eqMixin. *)
+Inductive lc_exp : exp -> Prop :=
+  | lc_tt : lc_exp tt
+  | lc_ff : lc_exp ff
+  | lc_one : lc_exp one
+  | lc_var a: lc_exp (V(EV.Free a))
+.
+Hint Constructors lc_exp.
 
-(* (* polarities have a simple order (e.g. + < -) *) *)
+Definition fv_exp (e : exp) : seq EV.atom :=
+  match e with
+    | V (EV.Free a) => [::a]
+    | _ => [::]
+  end.
 
-(* Definition ltn_pol (p p' : polarity) : bool := *)
-(*   match p, p' with *)
-(*   | Pos, Neg => true *)
-(*   | _, _ => false *)
-(*   end. *)
+(* Open a bound variable in an expression (original ope) *)
+Definition open_exp (n : nat) (e' : exp) (e : exp) : exp :=
+  match e with
+  | V v => EV.open_var V n e' v
+  | _ => e
+  end.
 
-(* Lemma ltn_pol_irreflexive : irreflexive ltn_pol. (* x : ltn_pol x x = false. *) *)
-(* Proof. *)
-(*     by case. *)
-(* Qed. *)
-
-(* Lemma ltn_pol_transitive : transitive ltn_pol. *)
-(* Proof. *)
-(*   by do !case. *)
-(* Qed. *)
-
-(* Lemma ltn_pol_total (a b : polarity) : [|| ltn_pol a b, a == b | ltn_pol b a]. *)
-(* Proof. *)
-(*   move: a b. *)
-(*   case ; case => //. *)
-(* Qed. *)
-
-(* Definition polarity_ordMixin : Ordered.mixin_of polarity_eqType := *)
-(*   OrdMixin *)
-(*     ltn_pol_irreflexive *)
-(*     ltn_pol_transitive *)
-(*     ltn_pol_total. *)
-(* Canonical Structure polarity_ordType := OrdType _ polarity_ordMixin. *)
-
-Definition channel := CH.var.
-(* Definition ch x p : channel := (x, p). *)
+(* processes *)
 
 Inductive proc : Set :=
-| send : channel -> exp -> proc -> proc
-| receive : channel -> proc -> proc
+| send : CH.var -> exp -> proc -> proc
+| receive : CH.var -> proc -> proc
 | ife : exp -> proc -> proc -> proc
 | par : proc -> proc -> proc
 | inact : proc
@@ -102,44 +85,25 @@ Hint Constructors proc.
 
 (**** locally nameless definitions ****)
 
-(* for expressions *)
-
-Inductive lc_exp : exp -> Prop :=
-  | lc_tt : lc_exp tt
-  | lc_ff : lc_exp ff
-  | lc_vare a: lc_exp (V(EV.Free a))
-.
-Hint Constructors lc_exp.
-
 (* free variables in things *)
 
-Definition fv_ch (k : channel) : seq CH.atom :=
-  match k with
-  | CH.Free a => [::a]
-  | _ => [::]
-  end.
-
-Definition fv_exp (e : exp) : seq EV.atom :=
-  match e with
-    | V (EV.Free a) => [::a]
-    | _ => [::]
-  end.
-
-Fixpoint fv_e (P : proc) : seq EV.atom :=
+(* original name fv_e *)
+(* may not be really needed *)
+Fixpoint fev_proc (P : proc) : seq EV.atom :=
   match P with
   | nu P
   | bang P
-  | receive _ P => fv_e P
-  | send _ e P => fv_exp e ++ fv_e P
-  | ife e P Q => fv_exp e ++ fv_e P ++ fv_e Q
-  | par P Q => fv_e P ++ fv_e Q
+  | receive _ P => fev_proc P
+  | send _ e P => fv_exp e ++ fev_proc P
+  | ife e P Q => fv_exp e ++ fev_proc P ++ fev_proc Q
+  | par P Q => fev_proc P ++ fev_proc Q
   | inact => [::]
   end.
 
 Fixpoint fv (P : proc) : seq CH.atom :=
   match P with
-  | send k e P => fv_ch k ++ fv P
-  | receive k P => fv_ch k ++ fv P
+  | send k e P => CH.fv k ++ fv P
+  | receive k P => CH.fv k ++ fv P
   | ife e P Q => fv P ++ fv Q
   | par P Q => fv P ++ fv Q
   | inact => [::]
@@ -147,19 +111,11 @@ Fixpoint fv (P : proc) : seq CH.atom :=
   | bang P => fv P
   end.
 
-
-(* Open a bound variable in an expression *)
-Definition ope (n : nat) (e' : exp) (e : exp) : exp :=
-  match e with
-  | V v => EV.open_var V n e' v
-  | _ => e
-  end.
-
 Fixpoint open_e (n : nat) (u : exp) (P : proc) : proc :=
   match P with
-  | send k e P => send k (ope n u e) (open_e n u P)
+  | send k e P => send k (open_exp n u e) (open_e n u P)
   | receive k P => receive k (open_e (S n) u P)
-  | ife e P Q => ife (ope n u e) (open_e n u P) (open_e n u Q)
+  | ife e P Q => ife (open_exp n u e) (open_e n u P) (open_e n u Q)
   | par P Q => par (open_e n u P) (open_e n u Q)
   | inact => inact
   | nu P => nu (open_e n u P)
@@ -169,14 +125,11 @@ Notation "{ope k ~> u } t" := (open_e k u t) (at level 67) : sr_scope.
 
 Open Scope sr_scope.
 Definition open_e0 P u :={ope 0~>u} P.
+(* this effectively substitutes variable index 0 with u *)
 
 (* for processes *)
 
-Inductive lc_ch : channel -> Prop :=
-| lc_channel a: lc_ch (CH.Free a).
-Hint Constructors lc_ch.
-
-Definition opk (n : nat) (u : CH.var) (k : channel) : channel :=
+Definition opk (n : nat) (u : CH.var) (k : CH.var) : CH.var :=
   CH.open_var id n u k.
 
 Fixpoint open_k (n : nat) (ko : CH.var) (P : proc) : proc :=
@@ -193,18 +146,15 @@ Notation "{opk k ~> u } t" := (open_k k u t) (at level 67) : sr_scope.
 
 Definition open_k0 P u :={opk 0~>u} P.
 
-(* TODO delete if not used *)
-(* Definition body P := forall (L : seq EV.atom) x, x \notin L -> lc (open_c0 P (LC.Free x)). *)
-
 Inductive lc : proc -> Prop :=
 | lc_send : forall k e P,
-    lc_ch k ->
+    CH.lc k ->
     lc_exp e ->
     lc P ->
     lc (send k e P)
 
 | lc_receive : forall (L : seq EV.atom) k P,
-    lc_ch k ->
+    CH.lc k ->
     (forall x, x \notin L -> lc (open_e0 P (V (EV.Free x)))) ->
     lc (receive k P)
 
@@ -225,6 +175,8 @@ Inductive lc : proc -> Prop :=
 | lc_bang P: lc P -> lc (bang P)
 .
 Hint Constructors lc.
+
+(* TODO what about lines 803-1346 SyntaxR.v *)
 
 (**** important definitions ****)
 
@@ -275,3 +227,43 @@ Inductive red_st : proc -> proc -> Prop :=
 | r_done P : P -->* P
 | r_step P Q R: P --> Q -> Q -->* R -> P -->* R
 where "P -->* Q" := (red_st P Q).
+
+
+(* substitutions when dealing with open terms (terms with names in them) *)
+
+Definition subst_ch (z : CH.atom) (k' : CH.var) (k : CH.var) : CH.var :=
+  if k == CH.Free z then k' else k.
+
+Definition subst_exp (z : EV.atom) (u : exp) (e : exp) : exp :=
+  match e with
+  | V (EV.Free b) => if z == b then u else e
+  | _ => e
+  end.
+
+Fixpoint subst_proc (z : CH.atom) (u : CH.var) (P : proc) : proc :=
+  match P with
+  | send k e P => send (subst_ch z u k) e (subst_proc z u P)
+  | receive k P => receive (subst_ch z u k) (subst_proc z u P)
+  | ife e P Q => ife e (subst_proc z u P) (subst_proc z u Q)
+  | par P Q => par (subst_proc z u P) (subst_proc z u Q)
+  | inact => inact
+  | nu P => nu (subst_proc z u P)
+  | bang P => bang (subst_proc z u P)
+  end.
+
+Fixpoint subst_proc_exp (z : EV.atom) (e : exp) (P : proc) : proc :=
+  match P with
+  | send k e' P => send k (subst_exp z e e') (subst_proc_exp z e P)
+  | receive k P => receive k (subst_proc_exp z e P)
+  | ife e' P Q => ife (subst_exp z e e') (subst_proc_exp z e P) (subst_proc_exp z e Q)
+  | par P Q => par (subst_proc_exp z e P) (subst_proc_exp z e Q)
+  | inact => inact
+  | nu P => nu (subst_proc_exp z e P)
+  | bang P => bang (subst_proc_exp z e P)
+  end.
+
+(* Notation "s[ z ~> u ]n a" := (subst_nm z u a) (at level 68) : sr_scope. *)
+Notation "s[ z ~> u ]c k" := (subst_ch z u k) (at level 68) : sr_scope.
+Notation "s[ z ~> u ]e e" := (subst_exp z u e) (at level 68) : sr_scope.
+Notation "s[ z ~> u ]p P" := (subst_proc z u P) (at level 68) : sr_scope.
+Notation "s[ z ~> e ]pe P" := (subst_proc_exp z e P) (at level 68) : sr_scope.
